examples/Sygus.v
@@ -20,15 +20,37 @@ Inductive res :=
 | N (n : nat)
 | B (b : bool).
 
+Inductive plus : nat -> nat -> nat -> Prop :=
+| plus0 n : plus 0 n n
+| plusS n m npm : plus n m npm -> plus (S n) m (S npm)
+.
+
+QuickChickDebug Debug On.
+
+Theorem plus_is_positive : forall n m npm, plus n m npm -> npm <= m.
+Proof.
+ (* quickchick.
+  QuickChick (sized theorem).*)
+  Extract Constant defNumTests => "100000".
+  Abort.
+
+Print checker.
+
+QuickChick checker.
+
+(*Derive Inductive Schedule plus 2 derive "Enum" opt "true".*)
+
+
 Inductive eval : exp -> nat -> nat -> res -> Prop :=
 | Eval_X : forall x y, eval X x y (N x)
 | Eval_Y : forall x y, eval Y x y (N y)                            
 | Eval_0 : forall x y, eval Zero x y (N 0)
 | Eval_1 : forall x y, eval One x y (N 1)
-(* | Eval_P : forall x y e1 e2 r1 r2,
+| Eval_P : forall x y e1 e2 r1 r2 r1p2,
     eval e1 x y (N r1) ->
-    eval e2 x y (N r2) ->                       
-    eval (P e1 e2) x y (N (r1 + r2)) (* Issue 1 *) *)
+    eval e2 x y (N r2) ->
+    plus r1 r2 r1p2 ->
+    eval (P e1 e2) x y (N r1p2) (* Issue 1 *)
 | Eval_ITE_T : forall x y e e1 e2 r,
     eval e x y (B true) ->
     eval e1 x y r ->
@@ -57,13 +79,20 @@ Derive Show for res.
 
 QuickChickDebug Debug Off.
 
-(*Derive Valid Schedules eval 0 consnum 8 derive "Gen".*)
+Derive Valid Schedules eval 0 consnum 6 derive "Gen".
 
 Derive Inductive Schedule eval 0 derive "Gen" opt "true".
 
-Print GenSizedSuchThateval_OIII.
+Derive Inductive Schedule eval 1 derive "Gen" opt "true".
 
-Derive ( Show) for exp.
+Sample (sized (fun n => GenSizedSuchThat_le_IO n 100)).
+
+Derive Show for exp.
+
+Sample (sized (fun n => GenSizedSuchThat_eval_OIII n 1 3 (N 4))).
+
+
+Print GenSizedSuchThat_le_IO.
 (*Derive Generator for (fun y => le x y).
 Derive Generator for (fun e => eval e x y r).*)
 
@@ -91,8 +120,22 @@ Fixpoint evalc (e : exp) (x y : nat) : option res :=
       | Some (N n1), Some (N n2) => Some (B (Nat.ltb n1 n2))
       | _, _ => None
       end
+  | P e1 e2 =>
+      match evalc e1 x y, evalc e2 x y with
+      | Some (N n1), Some (N n2) => Some (N (n1 + n2))
+      | _, _ => None
+      end
   | _ => None
   end.
+
+
+Instance DecEqRes : Dec_Eq res.
+Proof. dec_eq. Defined.
+
+Instance DecEqexp : Dec_Eq exp. dec_eq. Defined.
+
+Check (fun ( e : exp) => e = e ?).
+  
 
 Fixpoint partial_eval (e : exp) : exp :=
   match e with
@@ -114,12 +157,27 @@ Fixpoint partial_eval (e : exp) : exp :=
       | Zero, One => T
       | One, Zero => F
       | One, One => F
+      | P One x, P One y => Lt x y
+      | P x One, P One y => Lt x y
+      | P x One, P y One => Lt x y
+      | P One x, P y One => Lt x y
+    (*  | P One x, y => (if (x = y) ? then F else Lt (P One x) y)
+      | P x One, y => (if (x = y) ? then F else Lt (P x One) y)
+      | x, P One y => (if (x = y) ? then T else Lt x (P One y))
+      | x, P y One => (if (x = y) ? then T else Lt x (P y One))
+      | e1', e2' => (if (e1' = e2') ? then F else Lt e1' e2')*)
       | e1', e2' => Lt e1' e2'
+      end
+  | P e1 e2 =>
+      match partial_eval e1, partial_eval e2 with
+      | Zero, e2' => e2'
+      | e1', Zero => e1'
+      | e1', e2' => P e1' e2'
       end
   | _ => e
   end.
 
-Instance DecEqexp : Dec_Eq exp. dec_eq. Defined.
+Print partial_eval.
 
 Definition stuck (e : exp) : bool := (e = (partial_eval e)) ? . 
 
@@ -130,8 +188,6 @@ Definition shrinker e := if stuck e then [] else [partial_eval e].
 (*Definition g :=
   genSizedST (fun e => eval e 2 4 (N 4)).*)
 
-Instance DecEqRes : Dec_Eq res.
-Proof. dec_eq. Defined.
 
 Search shrink.
 
@@ -147,15 +203,14 @@ Definition forAllShrinkMaybe {A prop : Type} {_ : Checkable prop} `{Show A}
 
 Derive Inductive Schedule eval derive "Check" opt "true".
 
-Check DecOpteval_IIII.
-
+Derive Show for exp. 
 Definition prop (ts : list (nat * nat * res)) :=
   let genSize := 5 in
   let defElemIgnore := (0,0, N 0) in
   forAll (elems_ defElemIgnore ts) (fun '(x,y,r) =>
-  forAllShrinkMaybe (GenSizedSuchThateval_OIII genSize x y r) shrinker (fun e => 
+  forAllShrinkMaybe (GenSizedSuchThat_eval_OIII genSize x y r) shrinker (fun e => 
   negb (forallb (fun '(x,y,r) => 
-  match DecOpteval_IIII 10 e x y r
+  match DecOpt_eval_IIII 10 e x y r
                 with
   | Some true => true
   | _ => false
@@ -167,16 +222,20 @@ Definition test_cases : list (nat * nat * res) :=
 Extract Constant defNumTests => "100000". 
 QuickChick (prop test_cases).
 
-Print DecOpteval_IIII.
+Print DecOpt_eval_IIII.
 
-Derive Inductive Schedule eval 3 derive "Enum" opt "true".
-
+Derive Inductive Schedule eval 0 3 derive "Gen" opt "true".
+(*
 
 Compute (DecOpteval_IIII 10 ( (Lt One Zero)) 4 2 (B false)).
 Compute (DecOpteval_IIII 10 ( (T)) 4 2 (B false)).
-Print andBind.
+Print andBind.*)
 
-Inductive EVAL : res -> res -> exp -> Prop :=
+Merge (fun e => eval e x y r) With (fun e => eval e x' y' r') As EVAL.
+
+Derive Inductive Schedule EVAL 6 derive "Gen" opt "true".
+
+(*Inductive EVAL : res -> res -> exp -> Prop :=
   | Eval_Lt_FEval_Lt_F : forall  (e1' e2' : exp) (n1' n2' n1 n2 : nat),
                          n2' <= n1' ->
                          n2 <= n1 ->
@@ -219,12 +278,12 @@ Derive Inductive Schedule le 0 1 derive "Gen" opt "true". Print GenSizedSuchThat
 
 
 
-Derive Inductive Schedule EVAL 2 derive "Gen" opt "true".
+Derive Inductive Schedule EVAL 2 derive "Gen" opt "true".*)
 
 
 
 Inductive EVAL : nat -> nat -> res -> nat -> nat -> res -> exp -> Prop :=
-(*  | Eval_Lt_FEval_Lt_F : forall (x' y' : nat) (e1' e2' : exp) (n1' n2' x y n1 n2 : nat),
+  | Eval_Lt_FEval_Lt_F : forall (x' y' : nat) (e1' e2' : exp) (n1' n2' x y n1 n2 : nat),
                          n2' <= n1' ->
                          n2 <= n1 ->
                          EVAL x y (N n2) x' y' (N n2') e2' ->
@@ -243,7 +302,7 @@ Inductive EVAL : nat -> nat -> res -> nat -> nat -> res -> exp -> Prop :=
                          S n1' <= n2' ->
                          S n1 <= n2 ->
                          EVAL x y (N n2) x' y' (N n2') e2' ->
-                         EVAL x y (N n1) x' y' (N n1') e1' -> EVAL x y (B true) x' y' (B true) (Lt e1' e2') *)
+                         EVAL x y (N n1) x' y' (N n1') e1' -> EVAL x y (B true) x' y' (B true) (Lt e1' e2') 
   | Eval_FEval_F : forall x' y' x y : nat, EVAL x y (B false) x' y' (B false) F
   | Eval_TEval_T : forall x' y' x y : nat, EVAL x y (B true) x' y' (B true) T 
   | Eval_ITE_FEval_ITE_F : forall (x' y' : nat) (e' e1' e2' : exp) (r' : res) (x y : nat) (r : res),
@@ -259,13 +318,50 @@ Inductive EVAL : nat -> nat -> res -> nat -> nat -> res -> exp -> Prop :=
   | Eval_1Eval_1 : forall x' y' x y : nat, EVAL x y (N 1) x' y' (N 1) One
   | Eval_0Eval_0 : forall x' y' x y : nat, EVAL x y (N 0) x' y' (N 0) Zero 
   | Eval_YEval_Y : forall x' y' x y : nat, EVAL x y (N y) x' y' (N y') Y
-  | Eval_XEval_X : forall x' y' x y : nat, EVAL x y (N x) x' y' (N x') X .
+| Eval_XEval_X : forall x' y' x y : nat, EVAL x y (N x) x' y' (N x') X .
 
-Derive Inductive Schedule EVAL 6  derive "Enum" opt "true".
+Merge (fun e => EVAL x y r x' y' r' e) With (fun e => eval e x'' y'' r'') As EVAL'.
+
+Print EVAL'.
+
+Time Derive Inductive Schedule EVAL 6  derive "Enum" opt "true".
+
+
 
 Check EnumSizedSuchThatEVAL_IIIIIIO.
 
-Compute (EnumSizedSuchThatEVAL_IIIIIIO 30 2 4 (B true) 3 5 (B false)).
+Compute (EnumSizedSuchThatEVAL_IIIIIIO 2 4 2 (N 4) 3 5 (N 5)).
+
+Print EnumSizedSuchThatEVAL_IIIIIIO.
+
+Time Derive Inductive Schedule EVAL 6  derive "Gen" opt "true".
+
+
+
+Check GenSizedSuchThatEVAL_IIIIIIO.
+
+Sample (GenSizedSuchThatEVAL_IIIIIIO 2 4 2 (N 4) 3 5 (N 5)).
+
+Definition prop' (ts : list (nat * nat * res)) :=
+  let genSize := 5 in
+  let defElemIgnore := (0,0, N 0) in
+  forAll (elems_ defElemIgnore ts) (fun '(x,y,r) =>
+  forAll (elems_ defElemIgnore ts) (fun '(x',y',r') =>
+                                                                          
+  forAllShrinkMaybe (GenSizedSuchThatEVAL_IIIIIIO genSize x y r x' y' r') shrinker (fun e => 
+  negb (forallb (fun '(x,y,r) => 
+  match DecOpteval_IIII 10 e x y r
+                with
+  | Some true => true
+  | _ => false
+  end) ts)))).
+
+Definition test_cases' : list (nat * nat * res) :=
+  [ (4,2,N 4);(2,5,N 1);(1,1,N 1) ].
+
+Extract Constant defNumTests => "100000". 
+QuickChick (prop' test_cases').
+
 
 Merge (fun e => eval e x1 y1 r1) With (fun e => eval e x2 y2 r2) As EVAL.
 
